Projects/Util/Monad.lean
@@ -1,16 +1,20 @@
 import Projects.Util.List
 
 variable {α β γ : Type}
-variable {M : Type → Type} [hM : Monad M]
+variable {M : Type → Type} [hM : Monad M] [hM₂ : LawfulMonad M]
 
-def sequence_ (ms : List (M α)) : M Unit := do
+def sequence' (ms : List (M α)) : M Unit := do
   _ ← sequence ms
 
 def replicateM (n : ℕ) (m : M α) : M (List α) := do
   sequence # .replicate n m
 
-def replicateM_ (n : ℕ) (m : M α) : M Unit := do
-  sequence_ # .replicate n m
+def replicateM' (n : ℕ) (m : M α) : M Unit := do
+  sequence' # .replicate n m
+
+class MonadCnd (p : {α : Type} → M α → Prop) : Prop where
+  pure {α : Type} {x : α} : p (pure x)
+  bind {α β : Type} {m : M α} {f : α → M β} : p m → (∀ x, p (f x)) → p (m >>= f)
 
 -----
 
@@ -31,15 +35,67 @@ def gets (f : σ → α) : M α := do pure # f (←get)
 theorem run_run_snd {m₁ : StateM σ α} {m₂ : StateM σ β} {x : σ} :
 m₂.run (m₁.run x).2 = (do (λ _ => ()) <$> m₁; m₂).run x := rfl
 
-omit hσ in @[simp]
+omit hM₂ hσ in @[simp]
 theorem run_gets {f : σ → α} :
 StateT.run (@gets α (StateT σ M) _ σ _ f) =
 StateT.run (@get _ (StateT σ M) _ >>= λ x => pure (f x)) := rfl
 
-omit hσ in @[simp]
+omit hM₂ hσ in @[simp]
 theorem run_set {s : σ} : StateT.run (@set σ (StateT σ M) _ s) = λ _ => pure ((), s) := rfl
 
-omit hσ in @[simp]
+omit hM₂ hσ in @[simp]
 theorem run_set' {s : σ} : StateT.run (StateT.set s : StateT σ M Unit) = λ _ => pure ((), s) := rfl
 
 end MonadState
+
+omit hM₂ in @[simp]
+theorem sequence_nil : sequence ([] : List (M α)) = pure [] := rfl
+
+@[simp]
+theorem sequence_cons {m : M α} {ms} :
+sequence (m :: ms) = m >>= λ x => sequence ms >>= λ xs => pure (x :: xs) := by
+  unfold sequence; simp [traverse, List.traverse]; rw [←hM₂.bind_map]; simp
+
+@[simp]
+theorem sequence'_nil : sequence' ([] : List (M α)) = pure () := by
+  simp [sequence']
+
+@[simp]
+theorem sequence'_cons {m : M α} {ms} : sequence' (m :: ms) = m >>= λ _ => sequence' ms := by
+  simp [sequence']
+
+theorem MonadCnd.map {p} [H : MonadCnd p] {f : α → β} {m : M α} (h₁ : p m) : p (f <$> m) := by
+  rw [map_eq_pure_bind]; exact H.bind h₁ λ _ => H.pure
+
+theorem MonadCnd.sequence {p} [H : MonadCnd p] {ms : List (M α)}
+(h₁ : ∀ m ∈ ms, p m) : p (sequence ms) := by
+  induction ms <;> simp
+  · exact H.pure
+  nm m ms ih
+  simp at h₁
+  rcases h₁ with ⟨h₁, h₂⟩
+  exact H.bind h₁ λ _ => H.map # ih h₂
+
+theorem MonadCnd.sequence' {p} [H : MonadCnd p] {ms : List (M α)}
+(h₁ : ∀ m ∈ ms, p m) : p (sequence' ms) := by
+  unfold _root_.sequence'; simp; apply H.map # H.sequence h₁
+
+theorem MonadCnd.replicateM {p} [H : MonadCnd p] {m : M α} {n}
+(h₁ : p m) : p (replicateM n m) := by
+  apply H.sequence; simp [h₁]
+
+theorem MonadCnd.replicateM' {p} [H : MonadCnd p] {m : M α} {n}
+(h₁ : p m) : p (replicateM' n m) := by
+  apply H.sequence'; simp [h₁]
+
+namespace List
+
+variable {xs ys zs : List α}
+
+theorem mapM_eq_sequence {f : α → M β} : xs.mapM f = sequence (xs.map f) := by
+  induction xs <;> simp_all
+
+theorem forM_eq_sequence' {f : α → M Unit} : xs.forM f = sequence' (xs.map f) := by
+  induction xs <;> simp_all
+
+end List
